src/simple-proof/proof-stacks/Safety.v
@@ -3,42 +3,22 @@ Set Implicit Arguments.
 Require Import LibLN.
 Require Import Coq.Program.Equality.
 Require Import Definitions Weakening Narrowing Binding PreciseTypes Substitution CanonicalForms
-        RecordAndInertTypes InvertibleTypes GeneralToTight.
+        RecordAndInertTypes InvertibleTypes GeneralToTight OperationalSemantics.
 
-Reserved Notation "s1 '//' t1 '|->' s2 '//' t2" (at level 40, s2 at level 39).
-
-Inductive ec_red : trm -> ec -> trm -> ec -> Prop :=
-| red_sel : forall x m e t T ds,
-    binds x (val_new T ds) e ->
-    defs_has (open_defs x ds) (def_trm m t) ->
-    e // trm_sel (avar_f x) m |-> e // t
-| red_app : forall f a e T t,
-    binds f (val_lambda T t) e ->
-    e // trm_app (avar_f f) (avar_f a) |-> e // open_trm a t
-| red_let : forall v t s x,
-    x # s ->
-    s // trm_let (trm_val v) t |-> s & x ~ v // open_trm x t
-| red_let_var : forall t e x,
-    e // trm_let (trm_var (avar_f x)) t |-> e // open_trm x t
-| red_let_tgt : forall t0 t e t0' e',
-    e // t0 |-> e' // t0' ->
-    e // trm_let t0 t |-> e' // trm_let t0' t
-where "e1 // t1 |-> e2 // t2" := (ec_red t1 e1 t2 e2).
-
-Inductive sto_trm_typ : ec -> trm -> typ -> Prop :=
-| sto_trm_typ_c : forall G e t T,
+(** For the purposes of our evaluation semantics, a term is a
+ The typing of a term with a stack *)
+Inductive sta_trm_typ : sta * trm -> typ -> Prop :=
+| sta_trm_typ_c : forall G s t T,
     inert G ->
-    well_typed G e ->
+    well_typed G s ->
     G ⊢ t : T ->
-    sto_trm_typ e t T.
+    sta_trm_typ (s, t) T.
 
-Notation "'⊢' e ',' t ':' T" := (sto_trm_typ e t T) (at level 40, t at level 59).
+Hint Constructors sta_trm_typ.
 
-Inductive norm_form: trm -> Prop :=
-| nf_var: forall x, norm_form (trm_var x)
-| nf_val: forall v, norm_form (trm_val v).
+Notation "'⊢' t ':' T" := (sta_trm_typ t T) (at level 40, t at level 59).
 
-Hint Constructors norm_form.
+(** * Preservation *)
 
 (** If a value [v] has type [T], then [v] has a precise type [T']
     that is a subtype of [T].
@@ -52,120 +32,168 @@ Proof.
   destruct (IHty_trm _ eq_refl) as [T' [Hty Hsub]]. eauto.
 Qed.
 
-Lemma preservation_ty: forall G e t e' t' T,
-    well_typed G e ->
+(** Helper tactics for proving Preservation *)
+
+Ltac binds_eq :=
+  match goal with
+  | [Hb1: binds ?x _ ?G,
+     Hb2: binds ?x _ ?G |- _] =>
+     apply (binds_func Hb1) in Hb2; inversions Hb2
+  end.
+
+Ltac invert_red :=
+  match goal with
+  | [Hr: (_, _) |-> (_, _) |- _] => inversions Hr
+  end.
+
+Ltac solve_IH :=
+  match goal with
+  | [IH: well_typed _ _ ->
+         inert _ ->
+         forall t', (_, _) |-> (_, _) -> _,
+       Wf: well_typed _ _,
+       In: inert _,
+       Hr: (_, _) |-> (_, ?t') |- _] =>
+    specialize (IH Wf In t' Hr) as [G' [Hi [Hwt Ht']]]
+  end;
+  match goal with
+  | [Hi: _ & ?G' ⊢ _ : _ |- _] =>
+    exists G'; repeat split; auto
+  end.
+
+Ltac solve_let :=
+  invert_red; solve_IH; fresh_constructor; eauto; apply* weaken_rules.
+
+(** [s: G]                  #<br>#
+    [inert [G]              #<br>#
+    [(s, t) |-> (s', t')]   #<br>#
+    [G ⊢ t: T]              #<br>#
+    [―――――――――――――――――――]   #<br>#
+    [exists G', inert G']        #<br>#
+    [s': G, G']             #<br>#
+    [G, G' ⊢ t': T]         *)
+Lemma preservation_helper: forall G s t s' t' T,
+    well_typed G s ->
     inert G ->
-    e // t |-> e' // t' ->
+    (s, t) |-> (s', t') ->
     G ⊢ t : T ->
     exists G', inert G' /\
-          well_typed (G & G') e' /\
+          well_typed (G & G') s' /\
           G & G' ⊢ t' : T.
 Proof.
-  introv Hwf Hin Hred Ht.
-  gen t'.
-  dependent induction Ht; intros; try solve [inversions Hred].
-  - pose proof (canonical_forms_fun Hin Hwf Ht1) as [L [T' [t [Bis [Hsub Hty]]]]].
-    inversions Hred.
-    apply (binds_func H4) in Bis. inversions Bis.
+  introv Hwf Hin Hred Ht. gen t'.
+  dependent induction Ht; intros; try solve [invert_red].
+  - Case "ty_all_elim".
+    match goal with
+    | [Hx: _ ⊢ trm_var (avar_f _) : typ_all _ _ |- _] =>
+        pose proof (canonical_forms_fun Hin Hwf Hx) as [L [T' [t [Bis [Hsub Hty]]]]];
+          inversions Hred;
+          binds_eq
+    end.
     exists (@empty typ). rewrite concat_empty_r. repeat split; auto.
     pick_fresh y. assert (y \notin L) as FrL by auto. specialize (Hty y FrL).
     rewrite subst_intro_typ with (x:=y); auto.
     rewrite subst_intro_trm with (x:=y); auto.
     eapply subst_ty_trm; eauto. rewrite~ subst_fresh_typ.
-  - pose proof (canonical_forms_obj Hin Hwf Ht) as [S [ds [t [Bis [Has Ty]]]]].
-    inversions Hred.
-    apply (binds_func H1) in Bis. inversions Bis.
+  - Case "ty_new_elim".
+    pose proof (canonical_forms_obj Hin Hwf Ht) as [S [ds [t [Bis [Has Ty]]]]].
+    invert_red. binds_eq.
     exists (@empty typ). rewrite concat_empty_r. repeat split; auto.
-    rewrite <- (defs_has_inv Has H5). assumption.
-  - destruct t.
-    + inversions Hred; try solve [inversion H6].
-      pick_fresh y.
+    match goal with
+    | [Hd: defs_has _ (def_trm _ ?t') |- G ⊢ t': T] =>
+      rewrite* <- (defs_has_inv Has Hd)
+    end.
+  - Case "ty_let".
+    destruct t; try solve [solve_let].
+    + SCase "[t = let x = a in u] where a is a variable".
+      repeat invert_red. pick_fresh y.
       exists (@empty typ). rewrite concat_empty_r. repeat split; auto.
       rewrite subst_intro_trm with (x:=y); auto.
       rewrite <- subst_fresh_typ with (x:=y) (y:=x); auto.
       eapply subst_ty_trm; eauto. rewrite~ subst_fresh_typ.
-    + inversions Hred; try solve [inversion H6].
-      pose proof (well_typed_notin_dom Hwf H6).
+    + SCase "[t = let x = v in u] where v is a value".
+      repeat invert_red.
+      match goal with
+        | [Hn: ?x # ?s |- _] =>
+          pose proof (well_typed_notin_dom Hwf Hn) as Hng
+      end.
       pose proof (val_typing Ht) as [V [Hv Hs]].
-      pick_fresh y. assert (y \notin L) by auto.
-      specialize (H y H2).
+      pick_fresh y. assert (y \notin L) as Hy by auto.
+      specialize (H y Hy).
       exists (x ~ V). repeat split.
-      * rewrite <- concat_empty_l. constructor~.
-        apply (precise_inert_typ Hv).
-      * constructor~.
-        apply (precise_to_general Hv).
-      * rewrite subst_intro_trm with (x:=y); auto.
-        rewrite <- subst_fresh_typ with (x:=y) (y:=x); auto.
-        eapply subst_ty_trm; eauto.
-        { eapply weaken_rules; eauto. }
-        { apply~ fv_ctx_types_push. }
-        { rewrite~ subst_fresh_typ.
-          pose proof (ty_var (binds_tail x V G)).
-          apply (ty_sub H3). apply (weaken_subtyp Hs); eauto.
-        }
-    + inversions Hred.
-      specialize (IHHt Hwf Hin t0' H6) as [G' [Hin' [Hwf' Ht']]].
-      exists G'. repeat split; auto.
-      apply_fresh ty_let as z; eauto.
-      eapply weaken_rules; eauto.
-    + inversions Hred.
-      specialize (IHHt Hwf Hin t0' H6) as [G' [Hin' [Hwf' Ht']]].
-      exists G'. repeat split; auto.
-      apply_fresh ty_let as z; eauto.
-      eapply weaken_rules; eauto.
-    + inversions Hred.
-      specialize (IHHt Hwf Hin t0' H6) as [G' [Hin' [Hwf' Ht']]].
-      exists G'. repeat split; auto.
-      apply_fresh ty_let as z; eauto.
-      eapply weaken_rules; eauto.
-  - specialize (IHHt Hwf Hin t' Hred) as [G' [Hin' [Hwf' Ht']]].
-    exists G'. repeat split; auto.
-    apply weaken_subtyp with (G2:=G') in H.
-    + apply (ty_sub Ht' H).
-    + eauto.
+      ** rewrite <- concat_empty_l. constructor~. apply (precise_inert_typ Hv).
+      ** constructor~. apply (precise_to_general Hv).
+      ** rewrite subst_intro_trm with (x:=y); auto.
+         rewrite <- subst_fresh_typ with (x:=y) (y:=x); auto.
+         eapply subst_ty_trm; eauto.
+         { eapply weaken_rules; eauto. }
+         { apply~ fv_ctx_types_push. }
+         { rewrite~ subst_fresh_typ.
+           pose proof (ty_var (binds_tail x V G)).
+           eapply ty_sub. eauto. apply* weaken_subtyp. }
+  - Case "ty_sub".
+    solve_IH.
+    match goal with
+    | [Hs: _ ⊢ _ <: _,
+       Hg: _ & ?G' ⊢ _: _ |- _] =>
+      apply weaken_subtyp with (G2:=G') in Hs;
+      eauto
+    end.
 Qed.
 
-Theorem preservation : forall e e' t t' T,
-    ⊢ e, t : T ->
-    e // t |-> e' // t' ->
-    ⊢ e', t' : T.
+(** ** Preservation Theorem *)
+
+(** [⊢ (s, t): T]           #<br>#
+    [(s, t) |-> (s', t')]   #<br>#
+    [―――――――――――――――――――]   #<br>#
+    [⊢ (s', t'): T]         *)
+Theorem preservation : forall s s' t t' T,
+    ⊢ (s, t) : T ->
+    (s, t) |-> (s', t') ->
+    ⊢ (s', t') : T.
 Proof.
   introv Ht Hr. destruct Ht as [* Hi Hwf Ht].
-  lets Hp: (preservation_ty Hwf Hi Hr Ht). destruct Hp as [G' [Hi' [Hwf' Ht']]].
-  apply sto_trm_typ_c with (G:=G&G'); auto. apply* inert_concat.
+  lets Hp: (preservation_helper Hwf Hi Hr Ht). destruct Hp as [G' [Hi' [Hwf' Ht']]].
+  apply sta_trm_typ_c with (G:=G&G'); auto. apply* inert_concat.
 Qed.
 
-Theorem progress: forall e t T,
-    ⊢ e, t : T ->
-    norm_form t \/ exists e' t', e // t |-> e' // t'.
+(** * Progress *)
+
+(** Helper tactic for proving progress *)
+Ltac solve_let_prog :=
+  match goal with
+      | [IH: ⊢ (?s, ?t) : ?T ->
+             inert _ ->
+             well_typed _ _ -> _,
+         Hi: inert _,
+         Hwt: well_typed _ _ |- _] =>
+        assert (⊢ (s, t): T) as Hs by eauto;
+        specialize (IH Hs Hi Hwt) as [IH | [s' [t' Hr]]];
+        eauto; inversion IH
+      end.
+
+(** ** Progress Theorem *)
+
+(** [⊢ (s, t): T]           #<br>#
+    [(s, t) |-> (s', t')]   #<br>#
+    [―――――――――――――――――――]   #<br>#
+    [t] is in normal form   #<br>#
+    or [exists s', t'] such that [(s, t) |-> (s', t')] *)
+Theorem progress: forall s t T,
+    ⊢ (s, t) : T ->
+    norm_form t \/ exists s' t', (s, t) |-> (s', t').
 Proof.
-  introv Ht. destruct Ht as [* Hin Hwf Ht].
-  induction Ht; try solve [left; auto].
-  - pose proof (canonical_forms_fun Hin Hwf Ht1) as [L [T' [t [Bis [Hsub Hty]]]]].
-    right. exists e (open_trm z t).
-    eapply red_app; eauto.
-  - pose proof (canonical_forms_obj Hin Hwf Ht) as [S [ds [t [Bis [Has Ty]]]]].
-    right. exists e t.
-    eapply red_sel; eauto.
-  - right. destruct t.
-    + pose proof (var_typing_implies_avar_f Ht) as [x A]. subst.
-      exists e (open_trm x u). apply red_let_var.
+  introv Ht. inversion Ht as [G s' t' T' Hi Hwt HT]. subst.
+  induction HT; eauto.
+  - Case "ty_all_elim".
+    pose proof (canonical_forms_fun Hi Hwt HT1) as [L [T' [t [Bis [Hsub Hty]]]]].
+    right*.
+  - Case "ty_new_elim".
+    pose proof (canonical_forms_obj Hi Hwt HT) as [S [ds [t [Bis [Has Ty]]]]].
+    right*.
+  - Case "ty_let".
+    right. destruct t; try solve [solve_let_prog].
+    + pose proof (var_typing_implies_avar_f HT) as [x A]. subst*.
     + pick_fresh x.
-      exists (e & x ~ v) (open_trm x u).
-      eapply red_let; auto.
-    + specialize (IHHt Hin Hwf) as [IH | [e' [t' Hred]]].
-      * inversion IH.
-      * exists e' (trm_let t' u).
-        apply~ red_let_tgt.
-    + specialize (IHHt Hin Hwf) as [IH | [e' [t' Hred]]].
-      * inversion IH.
-      * exists e' (trm_let t' u).
-        apply~ red_let_tgt.
-    + specialize (IHHt Hin Hwf) as [IH | [e' [t' Hred]]].
-      * inversion IH.
-      * exists e' (trm_let t' u).
-        apply~ red_let_tgt.
-  - specialize (IHHt Hin Hwf) as [IH | [e' [t' Hred]]].
-    + left. assumption.
-    + right. exists e' t'. assumption.
+      exists (s & x ~ v) (open_trm x u). auto.
 Qed.
